src/lib/data/Kuiper.Matrix.Vectorized.fst
@@ -192,6 +192,7 @@ fn gpu_matrix_vec_read
   (#s : erased (seq et))
   preserves gpu
   preserves gm |-> Frac f em
+  requires  pure (aligned' 16 (core gm) (cell_of_pos l i j))
   requires  arr |-> s
   requires  pure (Pulse.Lib.Array.length arr >= chunk et)
   ensures   arr |-> Seq.init_ghost (chunk et) (fun x -> macc em i (j + x))
@@ -213,26 +214,4 @@ fn gpu_matrix_vec_read
   assert pure (Seq.equal s (Seq.init_ghost (chunk et) (fun x -> macc em i (j + x))));
 
   ();
-}
-
-inline_for_extraction noextract
-fn gpu_matrix_vec_read'
-  (#et:Type0) {| sized et, has_vec_cpy et |}
-  (#rows #cols : erased nat)
-  (#l : mlayout rows cols) {| clayout l, strided_row_major l |}
-  (gm : gpu_matrix et l)
-  (i : szlt rows)
-  (j : szlt (cols - chunk et + 1))
-  (#f : perm)
-  (#em : ematrix et rows cols)
-  (arr : array et)
-  (#s : erased (seq et))
-  preserves gpu
-  preserves gm |-> Frac f em
-  requires  arr |-> s
-  requires  pure (Pulse.Lib.Array.length arr >= chunk et)
-  ensures   exists* (s': lseq et (chunk et)). arr |-> s' **
-    pure (forall x. Seq.index s' x == macc em i (j + x))
-{
-  gpu_matrix_vec_read gm i j arr;
 }
