src/lib/poly/gemm/Kuiper.Poly.GEMM.BlockTiling2D.fst
@@ -70,7 +70,9 @@ let kpre1
   =
   gA |-> Frac (fA /. (rows/tm * (cols/tn))) eA **
   gB |-> Frac (fB /. (rows/tm * (cols/tn))) eB **
-  own_thread_tile gC bm bn tm tn bid tid
+  own_thread_tile gC bm bn tm tn bid tid **
+  pure (aligned 16 (core gA)) **
+  pure (aligned 16 (core gB))
 
 unfold
 let kpost1
@@ -837,6 +839,8 @@ fn mmcomb_gpu
     gA |-> Frac fA eA **
     gB |-> Frac fB eB
   requires
+    pure (aligned 16 (core gA)) **
+    pure (aligned 16 (core gB)) **
     pure (rows/bm * (cols/bn) <= max_blocks) **
     pure (bm/tm * (bn/tn) <= max_threads) **
     gC |-> eC
