src/lib/poly/gemm/Kuiper.Poly.GEMM.TensorCore2D.fst
@@ -520,6 +520,8 @@ let mk_kernel
   (#_ : squash (chunk et_ab /?+ bn))
   (#_ : squash (chunk et_ab /?+ bk))
   (#_: squash (SZ.fits (bm * bk) /\ SZ.fits (bk * bn)))
+  (#_ : squash (aligned 16 (core gA)))
+  (#_ : squash (aligned 16 (core gB)))
   (#fA #fB : perm)
   (nblk : szp{SZ.v nblk == rows/bm * (cols/bn)})
   (nthr : szp{SZ.v nthr == bm/(wm*tm) * (bn/(wn*tn)) * warp_size})
